src/program_proof/tulip/program/txn/txn_begin.v
@@ -1,32 +1,303 @@
+From Perennial.base_logic Require Import ghost_map saved_prop mono_nat.
+From Perennial.program_proof Require std_proof.
 From Perennial.program_proof.tulip.program Require Import prelude.
 From Perennial.program_proof.tulip.program.txn Require Import txn_repr.
 
+Local Ltac Zify.zify_post_hook ::= Z.div_mod_to_equations.
+
 Section program.
   Context `{!heapGS Σ, !tulip_ghostG Σ}.
+  Locate tulip_ghostG.
+
+  Local Definition zN_TXN_SITES : Z := 64.
+  Local Definition sid_of (ts: u64) : u64 := word.modu ts (W64 zN_TXN_SITES).
+
+  Definition sid_own (γ : tulip_names) (sid : u64) : iProp Σ :=
+    own γ.(sids) ({[ sid := Excl () ]}).
+
+  Local Definition gentid_au γ (sid : u64) (Φ : val → iProp Σ) : iProp Σ :=
+    (|NC={⊤ ∖ ↑tidNS,∅}=>
+      ∃ ts : nat, own_largest_ts γ ts ∗
+         (∀ ts' : nat, own_largest_ts γ ts' ∗ ⌜(ts < ts')%nat⌝ -∗
+           |NC={∅,⊤ ∖ ↑tidNS}=> ∀ tid : u64, ⌜uint.nat tid = ts'⌝ ∗ sid_own γ sid -∗ Φ #tid)).
+
+  Local Definition reserved_inv γ γr now (ts : u64): iProp Σ :=
+    ∃ Φ, let sid := sid_of ts in
+      saved_pred_own γr DfracDiscarded Φ ∗
+      sid_own γ sid ∗
+      if bool_decide (uint.nat ts ≤ now)%nat then
+        (* This ts has already happened *)
+        sid_own γ sid -∗ Φ #ts
+      else
+        (* This ts is still in the future *)
+        gentid_au γ sid Φ
+      .
+
+  Local Definition gentid_inv (γ : tulip_names) now : iProp Σ :=
+    ∃ prev (reserved : gmap u64 gname),
+      ⌜prev ≤ now⌝%nat ∗ own_largest_ts γ prev ∗ tsc_lb now ∗
+      ghost_map_auth γ.(gentid_reserved) 1 reserved ∗
+      [∗ map] ts ↦ 'γr ∈ reserved,
+        reserved_inv γ γr now ts.
+
+  Definition have_gentid (γ : tulip_names) : iProp Σ :=
+    inv tidNS (∃ now, gentid_inv γ now).
+
+  Local Definition tid_reserved γ γr ts (Φ : val → iProp Σ) : iProp Σ :=
+    ghost_map_elem γ.(gentid_reserved) ts (DfracOwn 1) γr ∗
+    saved_pred_own γr DfracDiscarded Φ.
+
+  Global Instance have_gentid_persistent γ : Persistent (have_gentid γ).
+  Proof. apply _. Qed.
+
+  Definition gentid_init γ : iProp Σ :=
+    own_largest_ts γ 0%nat ∗ ghost_map_auth γ.(gentid_reserved) 1 (∅ : gmap u64 gname).
+
+  Lemma init_GenTID γ E :
+    gentid_init γ -∗
+    |={E}=> have_gentid γ.
+  Proof.
+    iIntros "[Hts Hres]".
+    iMod tsc_lb_0.
+    iApply inv_alloc. iNext. iExists _, 0%nat, ∅.
+    iFrame. rewrite big_sepM_empty. eauto.
+  Qed.
+
+  Local Lemma gentid_reserve γ now sid Φ :
+    gentid_inv γ now -∗
+    sid_own γ sid -∗
+    gentid_au γ sid Φ -∗
+    |==> tsc_lb now ∗
+      (* The user can pick a timestamp with the right sid, but only gets something
+      out of this if they pick one that is strictly greater than [clock]. *)
+      (∀ ts, ⌜sid = sid_of ts⌝ ==∗
+         (if bool_decide (now < uint.Z ts) then ∃ γr, tid_reserved γ γr ts Φ else True) ∗
+         gentid_inv γ now).
+  Proof.
+    iIntros "(%last & %reserved & %Hlast & Hts & #Htsc & Hreserved_map & Hreserved) Hsid HAU".
+    iFrame "Htsc". iIntros "!> %ts %Hsid".
+    iAssert (⌜reserved !! ts = None⌝)%I as %Hfresh.
+    { destruct (reserved !! ts) as [γr|] eqn:Hts; last done. iExFalso.
+      iDestruct (big_sepM_lookup _ _ _ _ Hts with "Hreserved") as (Φ2) "(_ & Hsid2 & _)".
+      rewrite -Hsid.
+      iDestruct (own_valid_2 with "Hsid Hsid2") as %Hval. iPureIntro. move:Hval.
+      rewrite singleton_op singleton_valid. done. }
+    case_bool_decide; last first.
+    { (* They gave us an outdated timestamp. *)
+      iSplitR; first done. eauto with iFrame. }
+    iMod (saved_pred_alloc Φ DfracDiscarded) as (γr) "#HΦ"; first done.
+    iMod (ghost_map_insert ts γr with "Hreserved_map") as "[Hreserved_map Hreserved_ts]"; first done.
+    iSplitL "Hreserved_ts".
+    { rewrite /tid_reserved. eauto. }
+    iExists last, _. iFrame "Hreserved_map Hts". iSplitR; first done.
+    iApply big_sepM_insert; first done.
+    iFrame. rewrite /reserved_inv. rewrite bool_decide_false; last lia.
+    iExists Φ. iFrame "HΦ". rewrite -Hsid. iFrame. done.
+  Qed.
+
+  Local Lemma reserved_inc_clock γ now reserved :
+    reserved !! (W64 (S now)) = None →
+    ([∗ map] ts↦γr ∈ reserved, reserved_inv γ γr now ts) -∗
+    [∗ map] ts↦γr ∈ reserved, reserved_inv γ γr (S now) ts.
+  Proof.
+    intros Hnotnow.
+    iIntros "Hm". iApply (big_sepM_impl with "Hm").
+    iIntros "!> %ts %γr %Hts (%Φ & HΦ & Hsid & HAU)".
+    assert (uint.nat ts ≠ S now).
+    { intros Heq. rewrite -Heq in Hnotnow.
+      replace (W64 (uint.nat ts)) with ts in Hnotnow by word. congruence. }
+    iExists _. iFrame.
+    case_bool_decide.
+    - rewrite bool_decide_true. 2:lia. done.
+    - rewrite bool_decide_false. 2:lia. done.
+  Qed.
+
+  Local Lemma gentid_inc_clock γ old now :
+    (old ≤ now)%nat →
+    (now < 2^64) →
+    gentid_inv γ old -∗
+    tsc_lb now -∗
+    |NC={⊤∖↑tidNS}=> gentid_inv γ now.
+  Proof.
+    induction 1 using le_ind.
+    { eauto. }
+    iIntros (?) "Hgentid #Htsc".
+    iDestruct (IHle with "Hgentid [Htsc]") as ">Hgentid".
+    { lia. }
+    { iApply tsc_lb_weaken; last done. lia. }
+    iDestruct "Hgentid" as "(%last & %reserved & %Hlast & Hts & _ & Hreserved_map & Hreserved)".
+    set ts := S m.
+    destruct (reserved !! (W64 ts)) as [γr|] eqn:Hts; last first.
+    { (* Nothing reserved at this timestamp, not much to do. *)
+      iExists _, _. iFrame. iSplitR; first by eauto with lia.
+      iFrame "Htsc".
+      iApply reserved_inc_clock; done. }
+    (* Bump our timestamp. *)
+    iExists ts, _. iFrame. iFrame "Htsc".
+    iSplitR; first done.
+    rewrite !(big_sepM_delete _ _ _ _ Hts).
+    iDestruct "Hreserved" as "[Hthis Hreserved]".
+    rewrite !assoc. iSplitR "Hreserved"; last first.
+    { iApply reserved_inc_clock; last done.
+      rewrite lookup_delete. done. }
+    iDestruct "Hthis" as (Φ) "(HΦ & Hsid & HAU)".
+    rewrite bool_decide_false. 2:word.
+    iMod "HAU" as (ts') "[Hts' Hclose]".
+    rewrite /own_largest_ts.
+    iDestruct (mono_nat_auth_own_agree with "Hts Hts'") as %[_ <-].
+    iCombine "Hts Hts'" as "Hts".
+    iMod (mono_nat_own_update ts with "Hts") as "[[Hts $] _]".
+    { lia. }
+    iMod ("Hclose" with "[Hts]") as "Hfin".
+    { iFrame. eauto with lia. }
+    iModIntro. iExists _. iFrame. rewrite bool_decide_true.
+    2:word.
+    iIntros "Hsid". iApply "Hfin". iFrame. word.
+  Qed.
+
+  Local Lemma gentid_completed γ γr clock ts Φ :
+    £1 -∗
+    gentid_inv γ clock -∗
+    tid_reserved γ γr ts Φ -∗
+    tsc_lb (uint.nat ts) -∗
+    |NC={⊤∖↑tidNS}=> ∃ clock', gentid_inv γ clock' ∗ Φ #ts.
+  Proof.
+    iIntros "LC Hgentid Hreserved Htsc".
+    set clock' := max clock (uint.nat ts).
+    iAssert (|NC={⊤∖↑tidNS}=> gentid_inv γ clock')%I with "[Htsc Hgentid]" as ">Hgentid".
+    { destruct (decide (clock <= uint.nat ts)%nat); last first.
+      { replace clock' with clock by lia. done. }
+      iMod (gentid_inc_clock with "Hgentid Htsc") as "Hgentid"; first done.
+      { word. }
+      replace clock' with (uint.nat ts) by lia. done.
+    }
+    iDestruct "Hgentid" as "(%last & %reserved & %Hlast & Hts & #Htsc & Hreserved_map & Hreserved_all)".
+    iExists clock'.
+    iDestruct "Hreserved" as "[Hmap HΦ]".
+    iDestruct (ghost_map_lookup with "Hreserved_map Hmap") as %Hts.
+    iMod (ghost_map_delete with "Hreserved_map Hmap") as "Hreserved_map".
+    iDestruct (big_sepM_delete _ _ _ _ Hts with "Hreserved_all") as "[Hreserved Hreserved_all]".
+    iDestruct "Hreserved" as (Φ') "(HΦ' & Hsid & HAU)".
+    iDestruct (saved_pred_agree _ _ _ _ _ (#ts) with "HΦ HΦ'") as "EQ".
+    iMod (lc_fupd_elim_later with "LC EQ") as "EQ".
+    iRewrite "EQ". clear Φ.
+    rewrite bool_decide_true.
+    2:lia.
+    iModIntro. iSplitR "Hsid HAU".
+    - iExists _, _. iFrame. eauto.
+    - iApply "HAU". done.
+  Qed.
 
   Theorem wp_getTimestamp (sid : u64) γ :
-    ⊢
-    {{{ True }}}
+    uint.Z sid < zN_TXN_SITES →
+    ⊢ have_gentid γ -∗
+    {{{ sid_own γ sid }}}
     <<< ∀∀ (ts : nat), own_largest_ts γ ts >>>
-      getTimestamp #sid @ ↑tsNS
+      getTimestamp #sid @ ↑tidNS
     <<< ∃∃ (ts' : nat), own_largest_ts γ ts' ∗ ⌜(ts < ts')%nat⌝ >>>
-    {{{ (tid : u64), RET #tid; ⌜uint.nat tid = ts'⌝ }}}.
+    {{{ (tid : u64), RET #tid; ⌜uint.nat tid = ts'⌝ ∗ sid_own γ sid }}}.
   Proof.
-    iIntros (Φ) "!> _ HAU".
+  iIntros "%Hsid #Hinv !>" (Φ) "Hsid HAU".
     wp_rec.
+    rewrite /trusted_time.GetTime.
+    wp_pure_credit "LC".
+
 
     (*@ func getTimestamp(sid uint64) uint64 {                                  @*)
     (*@     ts := trusted_time.GetTime()                                        @*)
-    (*@                                                                         @*)
+    wp_apply (wp_GetTSC).
+    iInv "Hinv" as "Hgentid" "Hclose".
+    iMod (lc_fupd_elim_later with "LC Hgentid") as (clock) "Hgentid".
+    iMod (gentid_reserve with "Hgentid Hsid HAU") as "[Hclock Hcont]".
+    iApply ncfupd_mask_intro.
+    { solve_ndisj. }
+    iIntros "Hclose2".
+    iExists _. iFrame "Hclock".
+    iIntros (clock2) "[%Hclock Hclock2]".
+    iMod "Hclose2" as "_".
+    set inbounds := bool_decide (uint.Z clock2 + 64 < 2^64).
+    set clock2_boundsafe := if inbounds then clock2 else 0.
+    opose proof (u64_round_up_spec clock2_boundsafe (W64 64) _ _) as H.
+    { subst clock2_boundsafe inbounds. case_bool_decide; word. }
+    { word. }
+    move:H.
+    set rounded_ts := u64_round_up clock2_boundsafe (W64 64).
+    intros (Hmod & Hbound1 & Hbound2).
+    set reserved_ts := word.add rounded_ts sid.
+    assert ((uint.Z rounded_ts + uint.Z sid) `mod` 64 = uint.Z sid) as Hsidmod.
+    { rewrite Z.add_mod. 2:lia.
+      rewrite Hmod. rewrite [uint.Z sid `mod` _]Z.mod_small. 2:split;[word|done].
+      rewrite Z.mod_small. 1:lia. split;[word|done]. }
+    assert (uint.Z (sid_of reserved_ts) = uint.Z sid) as Hsid_of.
+    { rewrite /sid_of /reserved_ts.
+      rewrite word.unsigned_modu. 2:done.
+      rewrite word.unsigned_add. rewrite (wrap_small (_+_)). 2:word.
+      rewrite wrap_small. 1:done.
+      split.
+      - apply Z_mod_nonneg_nonneg. all:try word. all:done.
+      - trans (uint.Z zN_TXN_SITES). 2:done. apply Z.mod_pos_bound. done.
+    }
+    iMod ("Hcont" $! reserved_ts with "[]") as "[Hreserved Hgentid]".
+    { iPureIntro. rewrite /sid_of /reserved_ts. apply word.unsigned_inj. done. }
+    iMod ("Hclose" with "[Hgentid]") as "_".
+    { eauto. }
+    iIntros "!> _".
+
     (*@     n := params.N_TXN_SITES                                             @*)
+    wp_pures.
+
     (*@     tid := std.SumAssumeNoOverflow(ts, n) / n * n + sid                 @*)
+
+    wp_pures.
+    wp_apply std_proof.wp_SumAssumeNoOverflow. iIntros (Hoverflow).
+    assert (inbounds = true) as ->.
+    { subst inbounds. rewrite bool_decide_true; first done. word. }
+    subst clock2_boundsafe.
+    rewrite u64_Z_through_nat in Hclock.
+    rewrite bool_decide_true.
+    2:{ subst reserved_ts. word. }
+    iDestruct "Hreserved" as (γr) "Hreserved".
+    wp_pures.
+
+    set tid := (word.add _ _).
+    assert (tid = reserved_ts) as -> by done.
+    (*@                                                                         @*)
     (*@                                                                         @*)
     (*@     for trusted_time.GetTime() <= tid {                                 @*)
     (*@     }                                                                   @*)
-    (*@                                                                         @*)
-    (*@     return tid                                                          @*)
-    (*@ }                                                                       @*)
-  Admitted.
+
+    set P := λ (b : bool), (if b then True else tsc_lb (uint.nat reserved_ts))%I.
+    wp_apply (wp_forBreak_cond P with "[] []").
+    { clear Φ. iIntros "!> %Φ _ HΦ".
+      wp_apply (wp_GetTSC).
+      iMod tsc_lb_0 as "Htsc".
+      iApply ncfupd_mask_intro.
+      { solve_ndisj. }
+      iIntros "Hclose".
+      iExists _. iFrame "Htsc".
+      iIntros (new_time) "[%Htime Htsc]". iMod "Hclose" as "_".
+      iIntros "!> _". wp_pures.
+      case_bool_decide; wp_pures; iApply "HΦ"; unfold P.
+      - done.
+      - iApply tsc_lb_weaken; last done. lia.
+    }
+    { unfold P. auto. }
+    iIntros "Htsc". unfold P. clear P.
+
+    wp_pure_credit "LC1". wp_pure_credit "LC2".
+    iInv "Hinv" as "Hgentid" "Hclose".
+    iMod (lc_fupd_elim_later with "LC1 Hgentid") as (clock3) "Hgentid".
+    iMod (gentid_completed with "LC2 Hgentid Hreserved Htsc") as (clock4) "(Hgentid & HΦ)".
+    iMod ("Hclose" with "[Hgentid]") as "_".
+    { eauto. }
+    iModIntro.
+
+      (*@                                                                         @*)
+      (*@     return tid                                                          @*)
+      (*@ }                                                                       @*)
+
+    iApply "HΦ".
+  Qed.
 
   Theorem wp_Txn__begin (txn : loc) γ :
     ⊢ {{{ own_txn_uninit txn γ }}}
@@ -44,19 +315,26 @@ Section program.
     do 2 iNamed "Htxn". iNamed "Hsid".
     wp_loadField.
     wp_apply (wp_getTimestamp).
+    { admit. }
+    { admit. }
+    { admit. }
     iNamed "Hts".
+
+    (* Not sure which name space to use. *)
+    assert (↑tidNS = ↑tsNS) as ->.
+    { admit. }
     iMod "HAU" as (ts) "[Hts HAU]".
     iFrame "Hts".
     iIntros "!>" (ts') "[Hts %Hts]".
     iMod ("HAU" with "[$Hts]") as "HΦ"; first done.
     iModIntro.
-    iIntros (tidW HtidW).
+    iIntros (tidW) "(%Htidw&Hown)".
     wp_storeField.
     iApply "HΦ".
     iAssert (own_txn_ts txn ts')%I with "[$HtsW]" as "Hts"; first done.
     iFrame "∗ #".
     iPureIntro.
     rewrite /valid_ts. word.
-  Qed.
+  Admitted.
 
 End program.
